\chapter{Уравнения в полных дифференциалах}

\section{Задача 186}
\begin{gather}
  2yxdx - (x^2-y^2)dx = 0 \\
  \frac{\partial P}{\partial y}=\frac{\partial Q}{\partial x}=2x\implies \\
  U = dU = Pdx+Qdy \\
  dU=\frac{\partial U}{\partial x}dx + \frac{\partial U}{\partial y}dy\implies
  \left\{ \begin{aligned}
    \frac{\partial U}{\partial x} &= P = 2xy \\
    \frac{\partial U}{\partial y} &= Q = x^2 - y^2
  \end{aligned} \right. \\
  U = \int 2xydx+C(y)=x^2y + C(y) \\
  \frac{\partial x^2y+C(y)}{\partial y}=x^2-y^2\\
  x^2+C'(y)=x^2-y^2 \implies 
  C(y)=-\frac{y^3}{3}+\widetilde{C}\\
   \boxed{ U(x,y)=x^2y-\frac{y^3}{3}+\widetilde{C} }
\end{gather}


%%% Local Variables:
%%% mode: latex
%%% TeX-master: "rpz"
%%% End:

