\section{Задача 190}

\begin{gather}
\frac{3x^2+y^2}{y^2}dx -\frac{2x^3+5y}{y^3}dy=0\\
\frac{-2y(3x^2+y^2)+2yy^2}{y^2}=\frac{(-6x^2)y^3+3y^2(2x^2+5y)}{y^6}=\frac{\partial P}{\partial y}=\frac{\partial Q}{\partial x}\\
\left\{ \begin{aligned}
  \frac{\partial U}{\partial x} &= \frac{3x^2+y^2}{y^2}\implies U=\frac{1}{y^2}\int3x^2+y^2dx+C(y)  \\
  \frac{\partial U}{\partial y} &= -\frac{2x^3+5y}{y^3}  \rightrightarrows  \frac{\partial (\frac{1}{y^2}(x^3+y^2x)+C(y))}{\partial y}=-\frac{2x^3+5y}{y^3} 
\end{aligned} \right.\\
\Longrightarrow  C'(y)+0-\frac{2y(x^3)}{y^4}=-\frac{2x^3+5y}{y^3}\\
C'(y)=\frac{2x^3-2x^3+5y}{y^3}\Rightarrow C'(y)=\frac{5}{y^2}\\
C(y)=-5\frac{1}{y}+\widetilde C\longrightarrow \boxed{ U(x,y)=\frac{x^3}{y^2}+x-5\frac{1}{y}+\widetilde{C}}
\end{gather}


%%% Local Variables:
%%% mode: latex
%%% TeX-master: "rpz"
%%% End:
