\chapter{Уравнения не разрешённые относительно производной}
\section{Задача 251}

\begin{gather}
  y'^2xy=y^2+xy'\curvearrowleft \frac{d()}{dy'}\\
  \left\{ \begin{aligned}
     y'^2+xy&=y^2+xy   \\
    2y' & =x \rightarrow \frac{x^2}{4}+xy=y^2+\frac{x^2}{2} \curvearrowright 
  \end{aligned} \right.\\
  y^2-xy+\frac{x^2}{4}=0\rightarrowtail (y-\frac{x}{2})^2=0\dashrightarrow \boxed{y=\frac{x}{2}}\\
  y'^2+(xy-y^2)-xy'=0\to y'=\frac{x\pm \sqrt{x^2-4xy+4y^2}}{2}\\
  y'=x\pm(x-2y) \land   y'_1=\frac{x+(x-2y)}{2}\to \left\{
    \begin{aligned}
        x &\geqslant  2y \\
        x &< 2y
    \end{aligned}
\right\}\\
y'_1=x-y\to y'_1=y\\
y'+y=0\\
\int \frac{dy}{y}=-\int dx\\
y=C(x)e^{-x}\longrightarrow C'(x)e^{-x}-C(x)e^{-x}=x-C(x)e^{-x}\\
C'(x)=\frac{x}{e^{-x}}\longrightarrow \int e^xxdx=xe^x-\int e^xdx=ex(x-1)+\widetilde{C}\\
\Longrightarrow \swarrow \boxed{\mathcal{Y} =(e^x(x-1))e^{-x}}\\
\left[
    \begin{aligned}
        y&=C_2e^x \\
        y&=(x-1)+C_1e^X
    \end{aligned}    
\right.\\
\Downarrow \\
\left[
    \begin{aligned}
        y'&=\frac{x}{2}-\frac{1}{2} \\
        y&=\frac{x}{2}\to \left\{ \begin{aligned}
          x&=1\\
          y&= \frac{1}{2}
        \end{aligned} \right. \\
    \end{aligned}    
\right.
\end{gather}

%%% Local Variables:
%%% mode: latex
%%% TeX-master: "rpz"
%%% End:
