\section{Задача 426}

\begin{gather}
  yy''+1=y'^2 \\
  \text{Пусть } y' = p; y'' = pp' \\
  ypp' = p^2 -1 \\
  yp \frac{dp}{dy}=p^2-1 \\
  \frac{pdp}{p^2-1} = \frac{dy}{y} = \frac{2}{2} \frac{pdp}{p^2-1} = \frac{1}{2} \int \frac{dp^2-1}{p^2-1} \\
  \frac{1}{2} \ln p^2 - 1 = \ln y + C_1 \\
  \sqrt{p^2 - 1} = yC_1 \rightarrow p = \pm \sqrt{y^2C_1^2+1} \\
  \frac{dx}{dy} = \pm \sqrt{y^2 C_1^2 + 1} \\
  \begin{split}
    \pm \int \frac{du}{\sqrt{y^2C_1^2+1}} = \int dx = \frac{1}{C_1} \frac{dC_1y}{\sqrt{y^2 C_1}} \\
    \implies x + C_2 = \frac{1}{C_1} \ln |C_1 y + \sqrt{C_1y+1}|
  \end{split}
\end{gather}


%%% Local Variables:
%%% mode: latex
%%% TeX-master: "rpz"
%%% End:
